remove temporary and refactor all

Foundation/Modal/Neighborhood/Logic/E.lean
@@ -1,5 +1,15 @@
 import Foundation.Modal.Neighborhood.Hilbert
 import Foundation.Modal.Neighborhood.Completeness
+import Foundation.Modal.Neighborhood.Filtration
+import Foundation.Modal.Neighborhood.AxiomC
+import Foundation.Modal.Neighborhood.AxiomGeach
+import Foundation.Modal.Neighborhood.AxiomP
+import Foundation.Modal.Neighborhood.AxiomN
+
+
+@[simp]
+lemma Set.inter_eq_univ {s t : Set α} : s ∩ t = Set.univ ↔ s = Set.univ ∧ t = Set.univ := by
+  simpa using @Set.sInter_eq_univ _ {s, t};
 
 namespace LO.Modal
 
@@ -10,6 +20,7 @@ open Formula.Neighborhood
 
 namespace Neighborhood
 
+
 abbrev FrameClass.E : FrameClass := Set.univ
 
 protected abbrev Frame.simple_whitehole : Frame := ⟨Unit, λ _ => ∅⟩
@@ -18,9 +29,52 @@ protected abbrev Frame.simple_whitehole : Frame := ⟨Unit, λ _ => ∅⟩
 lemma Frame.simple_whitehole.not_valid_axiomN : ¬Frame.simple_whitehole ⊧ Axioms.N := by
   simp [Semantics.Realize, ValidOnFrame, ValidOnModel, Satisfies];
 
+
+section
+
+abbrev Frame.trivial_nontransitive : Frame := ⟨
+  Fin 2,
+  λ w =>
+    match w with
+    | 0 => ∅
+    | 1 => {Set.univ}
+⟩
+
+instance : Frame.trivial_nontransitive.IsRegular := by
+  constructor;
+  rintro X Y x ⟨hx, hy⟩;
+  match x with | 0 | 1 => simp_all;
+
+instance : Frame.trivial_nontransitive.IsMonotonic := by
+  constructor;
+  rintro X Y x; match x with | 0 | 1 => simp
+
+instance : Frame.trivial_nontransitive.IsReflexive := by
+  constructor;
+  rintro X x; match x with | 0 | 1 => first | tauto_set | simp_all;
+
+@[simp]
+lemma Frame.trivial_nontransitive.not_transitive : ¬Frame.trivial_nontransitive.IsTransitive := by
+  by_contra hC;
+  have := @(hC.trans Set.univ);
+  have := @this 1 ?_;
+  . have := Set.Subset.antisymm_iff.mp this |>.2;
+    have := @this 0;
+    simp at this;
+  . simp [Frame.box];
+
+@[simp]
+lemma Frame.trivial_nontransitive.not_valid_axiomFour : ¬Frame.trivial_nontransitive ⊧ Axioms.Four (.atom 0) := by
+  apply not_imp_not.mpr isTransitive_of_valid_axiomFour;
+  simp;
+
+end
+
 end Neighborhood
 
 
+
+namespace E
 
 instance : Sound Modal.E FrameClass.E := instSound_of_validates_axioms $ by simp;
 
@@ -29,6 +83,85 @@ instance : Entailment.Consistent Modal.E := consistent_of_sound_frameclass Frame
   simp;
 
 instance : Complete Modal.E FrameClass.E := minimalCanonicalFrame.completeness $ by tauto
+
+
+
+
+end E
+
+
+instance : Modal.E ⪱ Modal.EM := by
+  constructor;
+  . apply Hilbert.WithRE.weakerThan_of_subset_axioms;
+    simp;
+  . apply Entailment.not_weakerThan_iff.mpr;
+    use (Axioms.M (.atom 0) (.atom 1));
+    constructor;
+    . simp;
+    . apply Sound.not_provable_of_countermodel (𝓜 := FrameClass.E);
+      apply not_validOnFrameClass_of_exists_model_world;
+      let M : Model := {
+        World := Fin 3,
+        𝒩 := λ w =>
+          match w with
+          | 0 => {{1}}
+          | 1 => {{0}, {0, 1}}
+          | 2 => {{0}, {1, 2}},
+        Val := λ w =>
+          match w with
+          | 0 => {0, 1}
+          | 1 => {1, 2}
+          | _ => Set.univ
+      };
+      use M, 0;
+      constructor;
+      . tauto;
+      . simp! [M, Semantics.Realize, Satisfies];
+        ext x;
+        simp;
+        omega;
+
+instance : Modal.E ⪱ Modal.EC := by
+  constructor;
+  . apply Hilbert.WithRE.weakerThan_of_subset_axioms;
+    simp;
+  . apply Entailment.not_weakerThan_iff.mpr;
+    use Axioms.C (.atom 0) (.atom 1);
+    constructor;
+    . simp;
+    . apply Sound.not_provable_of_countermodel (𝓜 := FrameClass.E);
+      apply not_validOnFrameClass_of_exists_model_world;
+      let M : Model := {
+        World := Fin 2,
+        𝒩 := λ w =>
+          match w with
+          | 0 => {{0}, {1}}
+          | 1 => {∅},
+        Val := λ w =>
+          match w with
+          | 0 => {0}
+          | 1 => {1}
+          | _ => Set.univ
+      };
+      use M, 0;
+      constructor;
+      . tauto;
+      . simp [M, Semantics.Realize, Satisfies]
+
+instance : Modal.E ⪱ Modal.EN := by
+  constructor;
+  . apply Hilbert.WithRE.weakerThan_of_subset_axioms;
+    simp;
+  . apply Entailment.not_weakerThan_iff.mpr;
+    use Axioms.N
+    constructor;
+    . simp;
+    . apply Sound.not_provable_of_countermodel (𝓜 := FrameClass.E);
+      apply not_validOnFrameClass_of_exists_frame;
+      use Frame.simple_whitehole;
+      constructor;
+      . tauto;
+      . simp;
 
 instance : Modal.E ⪱ Modal.EK := by
   constructor;
@@ -64,19 +197,52 @@ instance : Modal.E ⪱ Modal.EK := by
           omega;
         . tauto_set;
 
-instance : Modal.E ⪱ Modal.EN := by
+instance : Modal.E ⪱ Modal.E4 := by
   constructor;
   . apply Hilbert.WithRE.weakerThan_of_subset_axioms;
     simp;
   . apply Entailment.not_weakerThan_iff.mpr;
-    use Axioms.N
+    use (Axioms.Four (.atom 0));
     constructor;
     . simp;
     . apply Sound.not_provable_of_countermodel (𝓜 := FrameClass.E);
       apply not_validOnFrameClass_of_exists_frame;
-      use Frame.simple_whitehole;
+      use Frame.trivial_nontransitive;
+      simp;
+
+instance : Modal.E ⪱ Modal.ED := by
+  constructor;
+  . apply Hilbert.WithRE.weakerThan_of_subset_axioms;
+    simp;
+  . apply Entailment.not_weakerThan_iff.mpr;
+    use (Axioms.D (.atom 0));
+    constructor;
+    . simp;
+    . apply Sound.not_provable_of_countermodel (𝓜 := FrameClass.E);
+      apply not_validOnFrameClass_of_exists_frame;
+      use ⟨Fin 2, λ w => match w with | 0 => {{0}} | 1 => Set.univ⟩
       constructor;
       . tauto;
-      . simp;
+      . apply not_imp_not.mpr isSerial_of_valid_axiomD;
+        by_contra! hC;
+        have := @hC.serial {1} 1;
+        simp [Frame.box, Frame.dia] at this;
+
+instance : Modal.E ⪱ Modal.EP := by
+  constructor;
+  . apply Hilbert.WithRE.weakerThan_of_subset_axioms;
+    simp;
+  . apply Entailment.not_weakerThan_iff.mpr;
+    use (Axioms.P);
+    constructor;
+    . simp;
+    . apply Sound.not_provable_of_countermodel (𝓜 := FrameClass.E);
+      apply not_validOnFrameClass_of_exists_frame;
+      use ⟨Fin 1, λ _ => {∅}⟩
+      constructor;
+      . tauto;
+      . apply not_imp_not.mpr notContainsEmpty_of_valid_axiomP;
+        by_contra! hC;
+        simpa using hC.not_contains_empty;
 
 end LO.Modal
