Foundation.lean
@@ -141,7 +141,6 @@ import Foundation.Modal.Neighborhood.Logic.E4
 import Foundation.Modal.Neighborhood.Logic.EMC4
 import Foundation.Modal.Neighborhood.Logic.EMCN
 import Foundation.Modal.Neighborhood.Logic.EMT4
-import Foundation.Modal.Neighborhood.Logic.EMCT4
 import Foundation.Modal.Neighborhood.Logic.END
 import Foundation.Modal.Neighborhood.Logic.ET4
 import Foundation.Modal.Neighborhood.Logic.Incomparability.ED_EP
