Foundation/Modal/Neighborhood/Logic/EMC.lean
@@ -1,6 +1,8 @@
+import Foundation.Modal.Neighborhood.AxiomGeach
 import Foundation.Modal.Neighborhood.Hilbert
-import Foundation.Modal.Neighborhood.Logic.EM
+import Foundation.Modal.Neighborhood.Logic.E4
 import Foundation.Modal.Neighborhood.Logic.EC
+import Foundation.Modal.Neighborhood.Logic.EM
 import Foundation.Vorspiel.Set.Fin
 
 
@@ -18,53 +20,6 @@ protected abbrev FrameClass.EMC : FrameClass := { F | F.IsEMC }
 
 instance : Frame.simple_whitehole.IsEMC where
   regular := by simp_all [Frame.simple_whitehole, Frame.box];
-
-abbrev EK_counterframe_for_M_and_C : Frame := {
-  World := Fin 4,
-  𝒩 := λ _ => {{0, 1}, {0, 2}}
-}
-
-lemma EK_counterframe_for_M_and_C.validate_axiomK : EK_counterframe_for_M_and_C ⊧ Axioms.K (atom 0) (atom 1) := by
-  intro V x;
-  apply Satisfies.def_imp.mpr;
-  intro h₁; replace h₁ := Satisfies.def_box.mp h₁;
-  apply Satisfies.def_imp.mpr;
-  intro h₂; replace h₂ := Satisfies.def_box.mp h₂;
-  apply Satisfies.def_box.mpr;
-  simp_all only [Fin.isValue, Model.truthset.eq_imp, Model.truthset.eq_atom, Set.mem_insert_iff, Set.mem_singleton_iff];
-  rcases h₂ with h₂ | h₂ <;> rcases h₁ with h₁ | h₁ <;>
-  . have := h₁.subset;
-    have := @this 3 $ by simp [h₂];
-    simp at this;
-
-lemma EK_counterframe_for_M_and_C.validate_axiomC : ¬EK_counterframe_for_M_and_C ⊧ Axioms.C (atom 0) (atom 1) := by
-  apply ValidOnFrame.not_of_exists_valuation_world;
-  use (λ a =>
-    match a with
-    | 0 => {0, 1}
-    | 1 => {0, 2}
-    | _ => ∅
-  ), 0;
-  simp [Satisfies];
-
-lemma EK_counterframe_for_M_and_C.validate_axiomM : ¬EK_counterframe_for_M_and_C ⊧ Axioms.M ((atom 0) ⋎ (atom 1)) (atom 1) := by
-  apply ValidOnFrame.not_of_exists_valuation_world;
-  use (λ a =>
-    match a with
-    | 0 => {0, 1}
-    | 1 => {0, 2}
-    | _ => ∅
-  ), 0;
-  suffices (({0, 2} : Set (Fin 4)) ⊆ {2, 0, 1}) ∧ ({2, 0, 1} : Set (Fin 4)) ≠ {0, 2} by
-    simp [Satisfies];
-    grind;
-  constructor;
-  . intro x;
-    simp only [Set.mem_insert_iff, Set.mem_singleton_iff];
-    tauto;
-  . by_contra hC;
-    have := hC.subset;
-    simpa using @this 1 (by simp)
 
 end Neighborhood
 
@@ -101,61 +56,19 @@ instance : Modal.EMC ⪱ Modal.EMCN := by
       . tauto;
       . simp;
 
-instance : Modal.EC ⪱ Modal.EMC := by
+instance : Modal.EMC ⪱ Modal.EMC4 := by
   constructor;
   . apply Hilbert.WithRE.weakerThan_of_subset_axioms;
     simp;
   . apply Entailment.not_weakerThan_iff.mpr;
-    use (Axioms.M (.atom 0) (.atom 1));
+    use (Axioms.Four (.atom 0));
     constructor;
     . simp;
-    . apply Sound.not_provable_of_countermodel (𝓜 := FrameClass.EC);
-      apply not_validOnFrameClass_of_exists_model_world;
-      let M : Model := {
-        World := Fin 3,
-        𝒩 := λ w =>
-          match w with
-          | 0 => {{1}}
-          | 1 => {{0}, {0, 1}}
-          | 2 => {{0}, {1, 2}, ∅},
-        Val := λ w =>
-          match w with
-          | 0 => {0, 1}
-          | 1 => {1, 2}
-          | _ => Set.univ
-      };
-      use M, 0;
+    . apply Sound.not_provable_of_countermodel (𝓜 := FrameClass.EMC);
+      apply not_validOnFrameClass_of_exists_frame;
+      use Frame.trivial_nontransitive;
       constructor;
-      . exact {
-          regular := by
-            rintro X Y w ⟨hwX, hwY⟩;
-            match w with
-            | 0 => simp_all [M];
-            | 1 =>
-              rcases hwX with (rfl | rfl) <;>
-              rcases hwY with (rfl | rfl) <;>
-              simp_all [M];
-            | 2 =>
-              rcases hwX with (rfl | rfl | rfl) <;>
-              rcases hwY with (rfl | rfl | rfl) <;>
-              simp [M]
-        }
-      . simp! [M, Semantics.Realize, Satisfies];
-        ext x;
-        simp!;
-        omega;
-
-instance : Modal.EK ⪱ Modal.EMC := by
-  constructor;
-  . apply Hilbert.WithRE.weakerThan_of_provable_axioms;
-    rintro φ rfl; simp;
-  . apply Entailment.not_weakerThan_iff.mpr;
-    use (Axioms.C (.atom 0) (.atom 1));
-    constructor;
-    . simp;
-    . apply not_imp_not.mpr $ soundness_of_axioms_validOnFrame (F := EK_counterframe_for_M_and_C) ?_;
-      . apply EK_counterframe_for_M_and_C.validate_axiomC;
-      . simp only [Semantics.RealizeSet.singleton_iff];
-        apply EK_counterframe_for_M_and_C.validate_axiomK;
+      . constructor;
+      . simp;
 
 end LO.Modal
