Foundation/Modal/Neighborhood/Logic/EMCN.lean
@@ -17,6 +17,9 @@ protected abbrev FrameClass.EMCN : FrameClass := { F | F.IsEMCN }
 
 end Neighborhood
 
+
+namespace EMCN
+
 instance : Sound Modal.EMCN FrameClass.EMCN := instSound_of_validates_axioms $ by
   constructor;
   rintro _ (rfl | rfl | rfl) F (rfl | rfl | rfl) <;> simp;
@@ -30,40 +33,7 @@ instance : Complete Modal.EMCN FrameClass.EMCN := maximalCanonicalFrame.complete
   apply Set.mem_setOf_eq.mpr;
   constructor;
 
-instance : Modal.ECN ⪱ Modal.EMCN := by
-  constructor;
-  . apply Hilbert.WithRE.weakerThan_of_subset_axioms;
-    simp;
-  . apply Entailment.not_weakerThan_iff.mpr;
-    use (Axioms.M (.atom 0) (.atom 1));
-    constructor;
-    . simp;
-    . apply Sound.not_provable_of_countermodel (𝓜 := FrameClass.ECN);
-      apply not_validOnFrameClass_of_exists_model_world;
-      let M : Model := {
-        World := Fin 2,
-        𝒩 := λ w => {∅, {0, 1}},
-        Val := λ w =>
-          match w with
-          | 0 => {0}
-          | 1 => {1}
-          | _ => Set.univ
-      };
-      use M, 0;
-      constructor;
-      . exact {
-          contains_unit := by
-            ext x;
-            match x with | 0 | 1 => simp_all [M, Set.Fin2.eq_univ];
-          regular := by
-            rintro X Y w ⟨hwX, hwY⟩;
-            simp_all only [Fin.isValue, Set.mem_setOf_eq, Set.mem_insert_iff, Set.mem_singleton_iff, M];
-            rcases hwX with (rfl | rfl) <;>
-            rcases hwY with (rfl | rfl) <;>
-            simp;
-        }
-      . simp! [M, Semantics.Realize, Satisfies];
-        tauto_set;
+end EMCN
 
 
 end LO.Modal
